FilteredRing/Exact.lean
@@ -1,0 +1,129 @@
+import FilteredRing.Test
+
+
+section exactness
+
+variable {ι R σ : Type*} [DecidableEq ι] [OrderedAddCommMonoid ι]
+  [Ring R] [SetLike σ R] [AddSubgroupClass σ R]
+
+variable (L M N : ι → σ) (L_lt M_lt N_lt : outParam <| ι → σ)
+  [IsRingFiltration L L_lt] [IsRingFiltration M M_lt] [IsRingFiltration N N_lt]
+
+variable (f : FilteredRingHom L L_lt M M_lt) (g : FilteredRingHom M M_lt N N_lt)
+
+
+open DirectSum DFinsupp
+
+
+theorem exact_of_strict_exact (fstrict : f.IsStrict) (gstrict : g.IsStrict)
+    (exact : Function.Exact f.toRingHom g.toRingHom) : Function.Exact (G f) (G g) := by
+  intro m
+  constructor
+  · have component_exact : ∀ p : ι, ∀ x : M p, (Gf g p) ⟦x⟧ = 0 → ∃ y : L p, (Gf f p) ⟦y⟧ = ⟦x⟧ := by
+      intro p x xto0
+      obtain⟨x', geq⟩ : ∃ x' : M_lt p, g.toRingHom x = g.toRingHom x' := by
+        simp only [Gf, GradedPiece.mk_eq, Quotient.lift_mk, QuotientAddGroup.eq_zero_iff] at xto0
+        have := (gstrict.strict_lt p (g.toRingHom x)).2 ⟨xto0, RingHom.mem_range_self g.toRingHom x⟩
+        rcases (Set.mem_image _ _ _).1 this with ⟨x', x'Mltp, geq⟩
+        use ⟨x', x'Mltp⟩, geq.symm
+
+      obtain⟨y, feq⟩ : ∃ y : L p, f.toRingHom y = x - x' := by
+        apply_fun (fun m ↦ m - g.toRingHom x') at geq
+        rw [sub_self, ← map_sub] at geq
+        replace strictf := fstrict.strict p (x - x') |>.2
+        have sub_mem_mp : x.1 - x' ∈ M p :=
+          sub_mem (SetLike.coe_mem x) <| (IsFiltration.lt_le M M_lt p) x'.2
+        replace strictf := strictf ⟨sub_mem_mp, (exact (x - x')).1 geq⟩
+        obtain ⟨y'', hy''⟩ := strictf
+        exact ⟨⟨y'', hy''.1⟩, hy''.2⟩
+
+      use y
+
+      have : (Gf f p) ⟦y⟧ = ⟦⟨f.toRingHom y, f.pieces_wise p y (SetLike.coe_mem y)⟩⟧ := by
+        simp only [Gf, GradedPiece.mk_eq, Quotient.lift_mk]
+      simp only [this, feq]
+      refine QuotientAddGroup.eq.mpr (AddSubgroup.mem_addSubgroupOf.mpr ?_)
+      simp only [AddSubgroup.coe_add, NegMemClass.coe_neg, neg_sub, sub_add_cancel, SetLike.coe_mem]
+
+    intro h
+    have h (i : ι): Gf g i (m i) = 0:= by
+      have : ((DirectSum.mk (GradedPiece N N_lt) (DFinsupp.support m)) fun i ↦ Gf g i (m ↑i)) i = 0 :=
+        (AddSemiconjBy.eq_zero_iff (((DirectSum.mk (GradedPiece N N_lt) <| DFinsupp.support m) fun i ↦ Gf g i (m ↑i)) i)
+        (congrArg (HAdd.hAdd (((DirectSum.mk (fun i ↦ GradedPiece N N_lt i) <| DFinsupp.support m) fun i ↦ Gf g i (m ↑i)) i))
+          (congrFun (congrArg DFunLike.coe <| id <| Eq.symm h) i))).mp rfl
+      rw [mk_eq_Gf M M_lt N N_lt g (x := m) (j := i)] at this
+      exact this
+
+    let component_1 := fun (i : ι) ↦ (if i ∈ support m then Classical.choose (Quotient.exists_rep (m i)) else 0)
+    have component_1_prop : ∀ i, ⟦component_1 i⟧ = m i := by
+      intro i
+      by_cases nh : i ∈ support m
+      · have : component_1 i = Classical.choose (Quotient.exists_rep (m i)) := if_pos nh
+        rw[this, Classical.choose_spec (Quotient.exists_rep (m i))]
+      · have : component_1 i = 0 := if_neg nh
+        simp only [mem_support_toFun, ne_eq, not_not] at nh
+        rw[this, nh]
+        rfl
+
+    have h : ∀ i, Gf g i ⟦component_1 i⟧ = 0 := by
+      intro i
+      rw[component_1_prop i, h i]
+
+    have tt (i : ι) : ∃ y, Gf f i ⟦y⟧ = m i := by
+      rw[← component_1_prop i]
+      exact component_exact i (component_1 i) (h i)
+
+    let component_2 := fun (i : support m) ↦ (⟦Classical.choose (tt i)⟧ : GradedPiece L L_lt i) --()
+    have (i : support m) :=  Gf f i (component_2 i)
+    have (i : support m): Gf f i (component_2 i) = m i := by
+      sorry
+      -- by_cases nh : i ∈ support m
+      -- · have : component_2 i = Classical.choose (tt i) := if_pos nh
+      --   rw[this, Classical.choose_spec (tt i)]
+      -- · have : component_2 i = 0 := if_neg nh
+      --   simp only [mem_support_toFun, ne_eq, not_not] at nh
+      --   rw[this, nh, Gf.mk L L_lt M M_lt f i 0]
+      --   simp only [Quotient.lift_mk, ZeroMemClass.coe_zero, map_zero, QuotientAddGroup.eq_zero_iff]
+      --   exact zero_mem (M_lt i)
+    let component_3 := fun (i : ι ) ↦ (if i ∈ support m then (⟦Classical.choose (tt i)⟧ : GradedPiece L L_lt i) else ⟦0⟧)
+
+    set s : AssociatedGraded L L_lt := DirectSum.mk (fun i ↦ GradedPiece L L_lt i) (support m) component_2 with hs
+
+    #check G f
+    -- have : s ∈  := sorry
+    have (i : support m): (G f) s i = m i := by
+
+      -- refine AssociatedGraded.ext_iff.mpr ?_
+      -- intro i
+      rw[← this i]
+      simp[G]
+      show ((DirectSum.mk (GradedPiece M M_lt) (support s)) fun i ↦ Gf f (↑i) (s ↑i)) ↑i = Gf f (↑i) (component_2 i)
+      #check mk_eq_Gf L L_lt M M_lt f (j := i) (x := s)
+      rw[ mk_eq_Gf L L_lt M M_lt f (j := i) (x := s)]
+      congr
+      rw[hs]
+      show ((DirectSum.mk (GradedPiece L L_lt) (support m)) component_2) i = component_2 i
+      #check mk_eq_Gf
+      -- rw?
+      -- rw[  L L_lt M M_lt f (j := i) (x := component_2)]
+      -- #check
+      -- rw[]
+      -- refine Eq.symm ((fun {ι} α [(i : ι) → Zero (α i)] {f} {i} {a} ↦ mem_singleton_apply_iff.mp) ?_)
+      sorry
+    -- #check mk _ component_2
+    sorry -- glue components together
+
+  · rintro ⟨l, hl⟩
+    rw[← hl]
+    show ((G g) ∘ (G f)) l = 0
+    rw[G.comp L L_lt M M_lt f N N_lt g]
+    ext i
+    obtain⟨k, hk⟩ : ∃ k, ⟦k⟧ = l i := Quotient.exists_rep (l i)
+    show ((DirectSum.mk (GradedPiece N N_lt) (DFinsupp.support l)) fun i ↦ Gf (g ∘ f) i (l i)) i = 0
+    rw [mk_eq_Gf L L_lt N N_lt (g ∘ f) (x := l) (j := i), Gf, ← hk, Quotient.lift_mk]
+    have : (⟨(g ∘ f).toRingHom k, by apply (g ∘ f).pieces_wise i k <| SetLike.coe_mem k⟩ : N i) = (0 : N i) :=
+      ZeroMemClass.coe_eq_zero.mp (Function.Exact.apply_apply_eq_zero exact k)
+    rw[this]
+    rfl
+
+end exactness
